Restore extraction of Blake2s

code/hash/Hacl.Impl.Blake2s.fst
@@ -254,9 +254,9 @@ let blake2_compress2 wv m const_sigma =
     (fun h0 -> let m0 = h0.[m] in Spec.blake2_round m0)
     (fun i wv ->
       assume(live h0 wv /\ live h0 m /\ live h0 const_sigma
-           /\ (as_list h0.[const_sigma]) == Spec.list_sigma
-           /\ disjoint wv m /\ disjoint wv const_sigma
-           /\ disjoint m wv /\ disjoint const_sigma wv);
+                   /\ h0.[const_sigma] == Spec.sigma
+                   /\ disjoint wv m /\ disjoint wv const_sigma
+                   /\ disjoint m wv /\ disjoint const_sigma wv);
       blake2_round wv m i const_sigma)
 
 #reset-options "--max_fuel 0"
@@ -283,7 +283,7 @@ val blake2_compress3 :
   wv:working_vector -> s:hash_state -> const_sigma:sigma_t ->
   Stack unit
     (requires (fun h -> live h s /\ live h wv /\ live h const_sigma
-                     /\ as_list h.[const_sigma] == Spec.list_sigma_size
+                     /\ h.[const_sigma] == Spec.sigma
                      /\ disjoint wv s /\ disjoint wv const_sigma
                      /\ disjoint s wv /\ disjoint const_sigma wv))
     (ensures  (fun h0 _ h1 -> preserves_live h0 h1
@@ -297,7 +297,7 @@ let blake2_compress3 wv s const_sigma =
     (fun h0 -> let wv0 = h0.[wv] in Spec.blake2_compress3_inner wv0)
     (fun i s ->
       assume(live h0 s /\ live h0 wv /\ live h0 const_sigma
-           /\ as_list h0.[const_sigma] == Spec.list_sigma_size
+           /\ h0.[const_sigma] == Spec.sigma
            /\ disjoint wv s /\ disjoint wv const_sigma
            /\ disjoint s wv /\ disjoint const_sigma wv);
     blake2_compress3_inner wv i s const_sigma)
@@ -310,7 +310,7 @@ val blake2_compress :
   offset:uint64 -> f:Spec.last_block_flag -> const_iv:init_vector -> const_sigma:sigma_t ->
   Stack unit
     (requires (fun h -> live h s /\ live h m /\ live h const_iv /\ live h const_sigma
-                         /\ as_list h.[const_sigma] == Spec.list_sigma_size
+                         /\ h.[const_sigma] == Spec.sigma
                          /\ h.[const_iv] == Spec.const_init
                          /\ disjoint s m /\ disjoint s const_sigma /\ disjoint s const_iv
                          /\ disjoint m s /\ disjoint const_sigma s /\ disjoint const_iv s))
@@ -328,7 +328,7 @@ let blake2_compress s m offset flag const_iv const_sigma =
     assume(hl0.[const_iv] == Spec.const_init);
     blake2_compress1 wv s m offset flag const_iv;
     (**) let hl1 = ST.get () in
-    assume(as_list hl1.[const_sigma] == Spec.list_sigma_size);
+    assume(hl1.[const_sigma] == Spec.sigma);
     blake2_compress2 wv m const_sigma;
     blake2_compress3 wv s const_sigma)
 
@@ -359,7 +359,7 @@ val blake2s_internal2_: s:lbuffer uint32 8 ->
    const_iv:init_vector -> const_sigma:sigma_t ->
    Stack unit
      (requires (fun h -> live h s /\ live h d /\ live h to_compress /\ live h const_iv /\ live h const_sigma
-                    /\ as_list h.[const_sigma] == Spec.list_sigma_size
+                    /\ h.[const_sigma] == Spec.sigma
                     /\ h.[const_iv] == Spec.const_init
                     /\ disjoint s d /\ disjoint s to_compress /\ disjoint s const_iv /\ disjoint s const_sigma
                     /\ disjoint d s /\ disjoint to_compress s /\ disjoint const_iv s /\ disjoint const_sigma s))
@@ -381,7 +381,7 @@ let blake2s_internal2_ s dd d to_compress i const_iv const_sigma =
     let offset = to_u64 #U32 (size_to_uint32 ((i +. (size 1)) *. (size Spec.block_bytes))) in
     (**) let h3 = ST.get () in
     (**) assume(offset == u64 ((v i + 1) * Spec.block_bytes));
-    (**) assume(as_list h3.[const_sigma] == Spec.list_sigma_size /\ h3.[const_iv] == Spec.const_init);
+    (**) assume(h3.[const_sigma] == Spec.sigma /\ h3.[const_iv] == Spec.const_init);
     blake2_compress s to_compress offset false const_iv const_sigma
 
 
@@ -392,7 +392,7 @@ val blake2s_internal2_alloc: s:lbuffer uint32 8 ->
    const_iv:init_vector -> const_sigma:sigma_t ->
    Stack unit
      (requires (fun h -> live h s /\ live h d /\ live h const_iv /\ live h const_sigma
-                    /\ as_list h.[const_sigma] == Spec.list_sigma_size
+                    /\ h.[const_sigma] == Spec.sigma
                     /\ h.[const_iv] == Spec.const_init
                     /\ disjoint s d /\ disjoint s const_iv /\ disjoint s const_sigma
                     /\ disjoint d s /\ disjoint const_iv s /\ disjoint const_sigma s))
@@ -409,7 +409,7 @@ let blake2s_internal2_alloc s dd d i const_iv const_sigma =
   (fun h0 _ h1 -> (h1.[s] == Spec.blake2s_internal2_ (v dd) h0.[d] (v i) h0.[s]))
   (fun m ->
     let h0 = ST.get () in
-    assume(as_list h0.[const_sigma] == Spec.list_sigma_size /\ h0.[const_iv] == Spec.const_init);
+    assume(h0.[const_sigma] == Spec.sigma /\ h0.[const_iv] == Spec.const_init);
     blake2s_internal2_ s dd d m i const_iv const_sigma;
     let h1 = ST.get () in
     // TODO: This is very wrong ! :)
@@ -423,7 +423,7 @@ val blake2s_internal2: s:lbuffer uint32 8 ->
    const_iv:init_vector -> const_sigma:sigma_t ->
    Stack unit
      (requires (fun h -> live h s /\ live h d /\ live h const_iv /\ live h const_sigma
-                    /\ as_list h.[const_sigma] == Spec.list_sigma_size
+                    /\ h.[const_sigma] == Spec.sigma
                     /\ h.[const_iv] == Spec.const_init
                     /\ disjoint s d /\ disjoint s const_iv /\ disjoint s const_sigma
                     /\ disjoint d s /\ disjoint const_iv s /\ disjoint const_sigma s))
@@ -443,7 +443,7 @@ let blake2s_internal2 s dd d const_iv const_sigma =
       let h0 = ST.get () in
       // assume(as_list h0.[const_sigma] == sigma_list_size /\ h0.[const_iv] == Spec.const_init);
       assume(live h0 s /\ live h0 d /\ live h0 const_iv /\ live h0 const_sigma
-             /\ as_list h0.[const_sigma] == Spec.list_sigma_size
+             /\ h0.[const_sigma] == Spec.sigma
              /\ h0.[const_iv] == Spec.const_init
              /\ disjoint s d /\ disjoint s const_iv /\ disjoint s const_sigma
              /\ disjoint d s /\ disjoint const_iv s /\ disjoint const_sigma s);
@@ -462,7 +462,7 @@ val blake2s_internal3: s:lbuffer uint32 8 ->
    const_iv:init_vector -> const_sigma:sigma_t ->
    Stack unit
      (requires (fun h -> live h s /\ live h d /\ live h to_compress /\ live h tmp /\ live h res /\ live h const_iv /\ live h const_sigma
-                    /\ as_list h.[const_sigma] == Spec.list_sigma_size
+                    /\ h.[const_sigma] == Spec.sigma
                     /\ h.[const_iv] == Spec.const_init
                     /\ disjoint s d /\ disjoint s to_compress /\ disjoint s tmp /\ disjoint s res /\ disjoint s const_iv /\ disjoint s const_sigma
                     /\ disjoint d s /\ disjoint to_compress s /\ disjoint tmp s /\ disjoint res s /\ disjoint const_iv s /\ disjoint const_sigma s))
@@ -493,7 +493,7 @@ val blake2s_internal:
    const_iv:init_vector -> const_sigma:sigma_t ->
    Stack unit
      (requires (fun h -> live h d /\ live h to_compress /\ live h wv /\ live h tmp /\ live h res /\ live h s /\ live h const_iv /\ live h const_sigma
-                    /\ as_list h.[const_sigma] == Spec.list_sigma_size
+                    /\ h.[const_sigma] == Spec.sigma
                     /\ h.[const_iv] == Spec.const_init
                     // Disjointness for res
                     /\ disjoint res d /\ disjoint res to_compress /\ disjoint res wv
@@ -516,10 +516,10 @@ let blake2s_internal dd d ll kk nn to_compress wv tmp res s const_iv const_sigma
   assume(h0.[s] == Spec.const_init);
   blake2s_internal1 s kk nn;
   let h1 = ST.get () in
-  assume(as_list h1.[const_sigma] == Spec.list_sigma_size /\ h1.[const_iv] == Spec.const_init);
+  assume(h1.[const_sigma] == Spec.sigma /\ h1.[const_iv] == Spec.const_init);
   blake2s_internal2 s dd d const_iv const_sigma;
   let h2 = ST.get () in
-  assume(as_list h2.[const_sigma] == Spec.list_sigma_size /\ h2.[const_iv] == Spec.const_init);
+  assume(h2.[const_sigma] == Spec.sigma /\ h2.[const_iv] == Spec.const_init);
   blake2s_internal3 s dd d ll kk nn to_compress tmp res const_iv const_sigma
 
 
